{-# OPTIONS --without-K  #-}


module GroupoidStructure where

open import Relation.Binary.PropositionalEquality 
open import Data.Product renaming (_,_ to _,,_)
open import Data.Nat


open import BasicSyntax renaming (_∾_ to htrans)
open import IdentityContextMorphisms
open import Suspension

Coh-rpl  : ∀{Γ Δ}(A : Ty Γ)(B : Ty Δ) → isContr Δ
         → Tm (rpl-T A B)
Coh-rpl {_} {Δ} A _ isC = coh (ΣC-it-ε-Contr A isC) _ _
refl*-Tm : Tm {x:*} (var v0 =h var v0)
refl*-Tm = Coh-Contr c*
sym*-Ty : Ty x:*,y:*,α:x=y
sym*-Ty = vY =h vX

sym*-Tm : Tm {x:*,y:*,α:x=y} sym*-Ty
sym*-Tm = Coh-Contr (ext c* v0)
trans*-Ty : Ty x:*,y:*,α:x=y,z:*,β:y=z
trans*-Ty = (vX +tm _ +tm _) =h vZ

trans*-Tm : Tm trans*-Ty
trans*-Tm = Coh-Contr (ext (ext c* v0) (vS v0))
refl-Tm    : {Γ : Con}(A : Ty Γ) 
           → Tm (rpl-T {Δ = x:*} A (var v0 =h var v0))
refl-Tm A  = rpl-tm A refl*-Tm

sym-Tm    : ∀ {Γ}(A : Ty Γ) → Tm (rpl-T A sym*-Ty)
sym-Tm A  = rpl-tm A sym*-Tm

trans-Tm    : ∀ {Γ}(A : Ty Γ) → Tm (rpl-T A trans*-Ty)
trans-Tm A  = rpl-tm A trans*-Tm

-- The version without lifting function

refl-Tm' :  {Γ : Con}(A : Ty Γ) → Tm {Γ , A} (var v0 =h var v0)
refl-Tm' A = (refl-Tm A)  [ map-1 ]tm ⟦ prf1 ⟫
  where
    prf : rpl-tm {Δ = x:*} A (var v0) [ map-1 ]tm ≅ var v0
    prf = htrans (congtm (htrans ([⊚]tm (Σtm-it A (var v0))) 
          (htrans (congtm (Σtm-it-p1 A)) (htrans wk-coh wk-coh+)))) 
           (1-1S-same-v0 (ΣT-it-p1 A))

    prf1 : (var v0 =h var v0) ≡ rpl-T {Δ = x:*} A (var v0 =h var v0) [ map-1 ]T
    prf1 = sym (trans (congT (rpl-T-p2 x:* A)) (hom≡ prf prf))

refl-Fun : (Γ : Con)(A : Ty Γ)(x : Tm A) → Tm (x =h x)
refl-Fun Γ A x =  (refl-Tm A) 
                 [ IdS , x ⟦ rpl*-A ⟫ ]tm 
                 ⟦ sym (trans (congT (rpl-T-p2 x:* A)) (hom≡ (rpl*-a A) (rpl*-a A))) ⟫

Tm-sym-fun : (Γ : Con)(A : Ty Γ) 
       → Tm (rpl-T  {Δ = ε , * , *} A (var (vS v0) =h var v0)) 
       → Tm (rpl-T  {Δ = ε , * , *} A (var v0 =h var (vS v0)))
Tm-sym-fun Γ A = fun (sym-Tm A ⟦ sym (rpl-T-p3 (ε , * , *) A) ⟫)

Tm-sym-fun2 : (Γ : Con)(A : Ty Γ) 
       → Tm {Γ , A , A +T A} (var (vS v0) =h var v0) 
       → Tm {Γ , A , A +T A} (var v0 =h var (vS v0))
Tm-sym-fun2 Γ A t =
  (t [ (wk-id , 
  (var v0 ⟦ eq1 ⟫)) ,
  (var (vS v0) ⟦ eq2 ⟫) ]tm)
  ⟦ sym (trans wk-hom (hom≡ (htrans (cohOp +T[,]T) 
    (cohOp eq1)) 
    (cohOp eq2))) ⟫

  where 
    wk-id : (Γ , A , A +T A) ⇒ Γ 
    wk-id = (IdS +S A) +S (A +T A)
  
    eq1 : A [ wk-id ]T ≡ (A +T A) +T (A +T A) 
    eq1 = wk+S+T (wk+S+T IC-T)

    eq2 : (A +T A) [ wk-id , (var v0 ⟦ eq1 ⟫) ]T 
            ≡ (A +T A) +T (A +T A) 
    eq2 = trans +T[,]T eq1

Fun-sym : (Γ : Con)(A : Ty Γ)(a b : Tm A) →
          Tm (a =h b)
       → Tm (b =h a)
Fun-sym Γ A a b t = (sym-Tm A) [ rpl-sub Γ A a b t ]tm 
         ⟦ sym (trans (rpl-T-p3-wk (ε , * , *) A) (trans (congT (rpl-T-p2 (ε , * , *) A)) 
           (hom≡ (rpl-tm-v0 (ε , *) A (cohOp (rpl*-A2 A))) (htrans (rpl-tm-vS (ε , *) A)
                 (rpl*-a A))))) ⟫



reflX : Tm (vX =h vX)
reflX = refl-Tm * +tm _ +tm _

reflY : Tm (vY =h vY)
reflY = refl-Tm * +tm _

m:*,n:*,α:m=n,p:*,β:n=p,q:*,γ:p=q : Con
m:*,n:*,α:m=n,p:*,β:n=p,q:*,γ:p=q = x:*,y:*,α:x=y,z:*,β:y=z , * , (var (vS (vS v0)) =h var v0)

vM : Tm {m:*,n:*,α:m=n,p:*,β:n=p,q:*,γ:p=q} *
vM = var (vS (vS (vS (vS (vS (vS v0))))))

vN : Tm {m:*,n:*,α:m=n,p:*,β:n=p,q:*,γ:p=q} *
vN = var (vS (vS (vS (vS (vS v0)))))

vMN : Tm {m:*,n:*,α:m=n,p:*,β:n=p,q:*,γ:p=q} (vM =h vN)
vMN = var (vS (vS (vS (vS v0))))

vP : Tm {m:*,n:*,α:m=n,p:*,β:n=p,q:*,γ:p=q} *
vP = var (vS (vS (vS v0)))

vNP : Tm {m:*,n:*,α:m=n,p:*,β:n=p,q:*,γ:p=q} (vN =h vP)
vNP = var (vS (vS v0))

vQ : Tm {m:*,n:*,α:m=n,p:*,β:n=p,q:*,γ:p=q} *
vQ = var (vS v0)

vPQ : Tm {m:*,n:*,α:m=n,p:*,β:n=p,q:*,γ:p=q} (vP =h vQ)
vPQ = var v0

Ty-G-assoc* : Ty m:*,n:*,α:m=n,p:*,β:n=p,q:*,γ:p=q
Ty-G-assoc* = (trans*-Tm [ ((((• , vM) , vP) , 
                       (trans*-Tm [ pr1 ⊚ pr1 ]tm)) , vQ) , vPQ ]tm =h 
             trans*-Tm [ (pr1 ⊚ pr1 ⊚ pr1 ⊚ pr1 , vQ) , 
                       (trans*-Tm [ ((((• , vN) , vP) , vNP) , vQ) , vPQ ]tm) ]tm)

Tm-right-identity* : 
  Tm {x:*,y:*,α:x=y} (trans*-Tm [ IdS , vY , reflY ]tm 
  =h vα)
Tm-right-identity* = Coh-Contr (ext c* v0)

Tm-left-identity* : 
  Tm {x:*,y:*,α:x=y} (trans*-Tm [ ((IdS ⊚ pr1 ⊚ pr1) , vX) ,
  reflX , vY , vα ]tm =h vα)
Tm-left-identity* = Coh-Contr (ext c* v0)

Tm-right-inverse* : 
  Tm {x:*,y:*,α:x=y} (trans*-Tm [ (IdS , vX) , sym*-Tm ]tm 
  =h reflX)
Tm-right-inverse* = Coh-Contr (ext c* v0)

Tm-left-inverse* : 
  Tm {x:*,y:*,α:x=y} (trans*-Tm [ ((• , vY) , vX , sym*-Tm ,
  vY) , vα ]tm =h reflY)
Tm-left-inverse* = Coh-Contr (ext c* v0)

Tm-G-assoc*  : Tm Ty-G-assoc*
Tm-G-assoc*  = Coh-Contr (ext (ext (ext c* v0) (vS v0)) 
             (vS v0))
Tm-G-assoc    : ∀{Γ}(A : Ty Γ) 
              → Tm (rpl-T A Ty-G-assoc*)
Tm-G-assoc A  = rpl-tm A Tm-G-assoc* 
